src/impl/TLS13.Impl.Handle.Dispatch.fsti
@@ -87,4 +87,5 @@ fn dispatch_network_event
                   (Ghost.reveal 'raw_bytes)
                   network_out_bytes
                   app_out_bytes /\
-                CT.some_legal_response 'st0 st1 resp network_out_bytes app_out_bytes)
+                CT.some_legal_response 'st0 st1 resp network_out_bytes app_out_bytes /\
+                (resp.CT.status == CT.NeedMoreInput ==> False))
